# baseURI: https://linked.data.gov.au/def/abis-msg

@prefix dcterms: <http://purl.org/dc/terms/> .
@prefix ex: <http://example.com/thing/> .
@prefix abism: <https://linked.data.gov.au/def/abis/> .
@prefix owl: <http://www.w3.org/2002/07/owl#> .
@prefix rdf: <http://www.w3.org/1999/02/22-rdf-syntax-ns#> .
@prefix rdfs: <http://www.w3.org/2000/01/rdf-schema#> .
@prefix skos: <http://www.w3.org/2004/02/skos/core#> .
@prefix sosa: <http://www.w3.org/ns/sosa/> .
@prefix tern: <https://w3id.org/tern/ontologies/tern/> .
@prefix time: <http://www.w3.org/2006/time#> .
@prefix void: <http://rdfs.org/ns/void#> .
@prefix xsd: <http://www.w3.org/2001/XMLSchema#> .

abism:DeleteObservationsMessage
  a owl:Class ;
  rdfs:label "Delete Observations Message" ;
  rdfs:subClassOf abism:GatewayMessage ;
  skos:definition "An RDF graph containing the identifiers of sosa:Observation instances to be deleted from the Biodiversity Data Repository"@en ;
  skos:prefLabel "Delete Observations Message"@en ;
.
abism:GatewayMessage
  a owl:Class ;
  rdfs:label "Gateway message" ;
  rdfs:subClassOf owl:Thing ;
.
abism:Message
  a owl:Class ;
  rdfs:label "Message" ;
  rdfs:subClassOf abism:GatewayMessage ;
  skos:definition "An RDF graph communicating instructions to the Biodiversity Data Repository's Gateway."@en ;
  skos:prefLabel "Message"@en ;
  skos:scopeNote "This is an abstract class and instances of it should not be created."@en ;
.
abism:NewObservationsMessage
  a owl:Class ;
  rdfs:label "New Observations Message" ;
  rdfs:subClassOf abism:GatewayMessage ;
  skos:definition "An RDF graph containing new tern:Observation instances indended to be stored in the Biodiversity Data Repository"@en ;
  skos:prefLabel "New Observations Message"@en ;
.
abism:UpdateObservationsMessage
  a owl:Class ;
  rdfs:label "Update Observations Message" ;
  rdfs:subClassOf abism:GatewayMessage ;
  skos:definition "An RDF graph containing tern:Observation instances already present in the Biodiversity Data Repository that are to be updated with this content"@en ;
  skos:prefLabel "Update Observations Message"@en ;
  skos:scopeNote "All originally supplied properties of the tern:Observation instances within the Biodiversity Data Repository will be deleted and then these new properties will be inserted. Properties of the tern:Observation instances calculated by the BDR may be recalculated."@en ;
.
<https://linked.data.gov.au/def/abis>
  a owl:Ontology ;
  rdfs:comment "An ontology for the Australian Australian Biodiversity Information Standard for Biodiversity Data (ABIS)"@en ;
  rdfs:label "ABIS Ontology"@en ;
.
