PREFIX : <https://linked.data.gov.au/dataset/bdr/smrr/>
PREFIX cs: <https://linked.data.gov.au/dataset/bdr/smrr>
PREFIX schema: <https://schema.org/>
PREFIX skos: <http://www.w3.org/2004/02/skos/core#>
PREFIX xsd: <http://www.w3.org/2001/XMLSchema#>

:IsolatedContent
    a skos:Concept ;
    skos:broader :ValidatableContent ;
    skos:definition "The Artifacts in this Resource contain content that can only be validated after loading the Resource with role NecessaryForValidation"@en ;
    skos:historyNote "Defined by BDR Staff for use in data submissions to the BDR" ;
    skos:inScheme cs: ;
    skos:prefLabel "Isolated Content"@en ;
    skos:topConceptOf cs: ;
.

:NecessaryForValidation
    a skos:Concept ;
    skos:definition "The Artifacts in this Resource must be loaded before other Resources are validated. These resources are not expected to be valid by themselves as they may contain no data"@en ;
    skos:historyNote "Defined by BDR Staff for use in data submissions to the BDR" ;
    skos:inScheme cs: ;
    skos:prefLabel "Necessary For Validation"@en ;
    skos:topConceptOf cs: ;
.

:NecessaryForValidation-External
    a skos:Concept ;
    skos:broader :NecessaryForValidation ;
    skos:definition "The Artifacts in this Resource must be loaded before other Resources are validated. These Resources are stored externally to the main content of the Manifest defining this Resource"@en ;
    skos:historyNote "Defined by BDR Staff for use in data submissions to the BDR" ;
    skos:inScheme cs: ;
    skos:prefLabel "Necessary For Validation - External"@en ;
.

:SubmissionSourceArchive
    a skos:Concept ;
    skos:broader :NotForValidation ;
    skos:definition "The Artifacts in this Resource are source data for the Submission defined by the Manifest defining this Resource. They must not be validated"@en ;
    skos:historyNote "Defined by BDR Staff for use in data submissions to the BDR" ;
    skos:inScheme cs: ;
    skos:prefLabel "Submission Source Archive"@en ;
    skos:topConceptOf cs: ;
.

:SufficientForValidation
    a skos:Concept ;
    skos:broader :ValidatableContent ;
    skos:definition "The Artifacts in this Resource can be validated after loading. No other Resources are necissary"@en ;
    skos:historyNote "Defined by BDR Staff for use in data submissions to the BDR" ;
    skos:inScheme cs: ;
    skos:prefLabel "Sufficient For Validation"@en ;
    skos:topConceptOf cs: ;
.

:SupplimentaryData
    a skos:Concept ;
    skos:broader :NotForValidation ;
    skos:definition "The Artifacts in this Resource are supplimentary, non-RDF, data for the Submission defined by the Manifest defining this Resource. They must not be validated"@en ;
    skos:historyNote "Defined by BDR Staff for use in data submissions to the BDR" ;
    skos:inScheme cs: ;
    skos:prefLabel "Supplimentary Data"@en ;
    skos:topConceptOf cs: ;
.

:NotForValidation
    a skos:Concept ;
    skos:definition "The Artifacts in this Resource must not be validated"@en ;
    skos:historyNote "Defined by BDR Staff for use in data submissions to the BDR" ;
    skos:inScheme cs: ;
    skos:prefLabel "Not For Validation"@en ;
    skos:topConceptOf cs: ;
.

:ValidatableContent
    a skos:Concept ;
    skos:definition "The Artifacts in this Resource must be validated"@en ;
    skos:historyNote "Defined by BDR Staff for use in data submissions to the BDR" ;
    skos:inScheme cs: ;
    skos:prefLabel "Validatable Content"@en ;
    skos:topConceptOf cs: ;
.

cs:
    a skos:ConceptScheme ;
    skos:definition "The roles that resources plan in BDR Submission Manifests"@en ;
    skos:historyNote "This vocabulary was developed to assist with the processing of data submissions to the Biodiversity Data Repository in February 2025" ;
    skos:prefLabel "BDR Submission Manifest Resource Roles"@en ;
    skos:scopeNote "See the ABIS Specification, <https://linked.data.gov.au/def/abis> - BDR Profile Section, for the definition of BDR Submission Manifests"@en ;
    schema:creator <https://linked.data.gov.au/org/dcceew> ;
    schema:dateCreated "2025-02-10"^^xsd:date ;
    schema:dateModified "2025-02-10"^^xsd:date ;
    schema:license <http://purl.org/NET/rdflicense/cc-by4.0> ;
    schema:publisher <https://linked.data.gov.au/org/dcceew> ;
    skos:hasTopConcept
        :NecessaryForValidation ,
        :SufficientForValidation ,
        :NotForValidation ,
        :ValidatableContent ;
.